@prefix : <http://www.semanticweb.org/luciapifferi/ontologies/2020/semantic_web_exam/narratives#> .
@prefix owl: <http://www.w3.org/2002/07/owl#> .
@prefix rdf: <http://www.w3.org/1999/02/22-rdf-syntax-ns#> .
@prefix xml: <http://www.w3.org/XML/1998/namespace> .
@prefix xsd: <http://www.w3.org/2001/XMLSchema#> .
@prefix rdfs: <http://www.w3.org/2000/01/rdf-schema#> .
@base <http://www.semanticweb.org/luciapifferi/ontologies/2020/semantic_web_exam/narratives> .

<http://www.semanticweb.org/luciapifferi/ontologies/2020/semantic_web_exam/narratives> rdf:type owl:Ontology .

#################################################################
#    Object Properties
#################################################################

###  http://www.semanticweb.org/luciapifferi/ontologies/2020/semantic_web_exam/narratives#collaborates
:collaborates rdf:type owl:ObjectProperty ;
              owl:inverseOf :collaborates ;
              rdf:type owl:SymmetricProperty ;
              rdfs:domain [ rdf:type owl:Class ;
                            owl:unionOf ( :Narrator
                                          :Publisher
                                        )
                          ] ;
              rdfs:range [ rdf:type owl:Class ;
                           owl:unionOf ( :Narrator
                                         :Publisher
                                       )
                         ] ;
              owl:propertyChainAxiom ( :creates
                                       :isReportedIn
                                       :hasPublisher
                                     ) ;
              rdfs:comment """if a narrator creates a narrative that is reported in a book that is published by a publisher, then the narrator collaborates with that publisher. 
This object property links narrator to publisher."""@en ;
              rdfs:label "collaborates"@en .


###  http://www.semanticweb.org/luciapifferi/ontologies/2020/semantic_web_exam/narratives#compose
:compose rdf:type owl:ObjectProperty ;
         owl:inverseOf :isComposedOf ;
         rdfs:domain :Event ;
         rdfs:range :Narrative ;
         rdfs:comment """An event composes a narrative. This property is not functional because, in my conceptualization, the same event can compose more narratives. 
This object property links events to narrative(s)."""@en ;
         rdfs:label "composes"@en .


###  http://www.semanticweb.org/luciapifferi/ontologies/2020/semantic_web_exam/narratives#creates
:creates rdf:type owl:ObjectProperty ;
         owl:inverseOf :isCreatedBy ;
         rdfs:domain :Narrator ;
         rdfs:range :Narrative ;
         rdfs:comment """One or more narrator create a narrative. It's reasonable to think that a narrator can create more than one narrative, so this property is not functional.
This object property links narrator and narrative(s)."""@en ;
         rdfs:label "creates"@en .


###  http://www.semanticweb.org/luciapifferi/ontologies/2020/semantic_web_exam/narratives#hasCharacter
:hasCharacter rdf:type owl:ObjectProperty ;
              rdfs:subPropertyOf :hasParticipant ;
              owl:inverseOf :isCharacterOf ;
              rdfs:domain :Event ;
              rdfs:range :Character ;
              owl:propertyDisjointWith :hasObject ;
              rdfs:comment "An event can have one or more characters as participants. This object property links event to character(s)."@en ;
              rdfs:label "hasCharacter"@en .


###  http://www.semanticweb.org/luciapifferi/ontologies/2020/semantic_web_exam/narratives#hasObject
:hasObject rdf:type owl:ObjectProperty ;
           rdfs:subPropertyOf :hasParticipant ;
           owl:inverseOf :isObjectOf ;
           rdfs:domain :Event ;
           rdfs:range :Object ;
           rdfs:comment "An event can have one or more objects as participants. This object property links event to object(s)."@en ;
           rdfs:label "hasObject"@en .


###  http://www.semanticweb.org/luciapifferi/ontologies/2020/semantic_web_exam/narratives#hasParticipant
:hasParticipant rdf:type owl:ObjectProperty ;
                owl:inverseOf :isParticipantOf ;
                rdfs:domain :Event ;
                rdfs:range :Participant ;
                rdfs:comment """Each event has at least one participating character or object. 
Since an event can have multiple participants, this property is not functional.
This object property links event and partcipant(s)."""@en ;
                rdfs:label "hasParticipant"@en .


###  http://www.semanticweb.org/luciapifferi/ontologies/2020/semantic_web_exam/narratives#hasPublisher
:hasPublisher rdf:type owl:ObjectProperty ;
              owl:inverseOf :isPublisherOf ;
              rdf:type owl:FunctionalProperty ;
              rdfs:domain :Book ;
              rdfs:range :Publisher ;
              rdfs:comment """A book has exactly one publisher, so this property is functional. 
This object property links book to publisher."""@en ;
              rdfs:label "hasPublisher"@en .


###  http://www.semanticweb.org/luciapifferi/ontologies/2020/semantic_web_exam/narratives#hosts
:hosts rdf:type owl:ObjectProperty ;
       owl:inverseOf :occursIn ;
       rdf:type owl:InverseFunctionalProperty ;
       rdfs:domain :Location ;
       rdfs:range :Event ;
       rdfs:comment "A location can host more than one event, but an event occurs in exactly one location. So this object property is inverse functional and links location and event(s)."@en ;
       rdfs:label "hosts"@en .


###  http://www.semanticweb.org/luciapifferi/ontologies/2020/semantic_web_exam/narratives#isCharacterOf
:isCharacterOf rdf:type owl:ObjectProperty ;
               rdfs:subPropertyOf :isParticipantOf ;
               rdfs:domain :Character ;
               rdfs:range :Event ;
               owl:propertyDisjointWith :isObjectOf ;
               rdfs:comment """A character can be the character of one ore more events.
This object property links character to event(s)."""@en ;
               rdfs:label "isCharacterOf"@en .


###  http://www.semanticweb.org/luciapifferi/ontologies/2020/semantic_web_exam/narratives#isComposedOf
:isComposedOf rdf:type owl:ObjectProperty ;
              rdfs:domain :Narrative ;
              rdfs:range :Event ;
              rdfs:comment """A narrative is exclusively composed of one or more events.
This object property links a narrative and event(s)."""@en ;
              rdfs:label "isComposedOf"@en .


###  http://www.semanticweb.org/luciapifferi/ontologies/2020/semantic_web_exam/narratives#isCreatedBy
:isCreatedBy rdf:type owl:ObjectProperty ;
             rdfs:domain :Narrative ;
             rdfs:range :Narrator ;
             rdfs:comment """Each narrative is created by at least one narrator. Since more than one narrator can create a narrative, this property is not functional.
This object property links narrative and narrator(s)."""@en ;
             rdfs:label "isCreatedBy"@en .


###  http://www.semanticweb.org/luciapifferi/ontologies/2020/semantic_web_exam/narratives#isObjectOf
:isObjectOf rdf:type owl:ObjectProperty ;
            rdfs:subPropertyOf :isParticipantOf ;
            rdfs:domain :Object ;
            rdfs:range :Event ;
            rdfs:comment """An object can be the object of one ore more events.
This object property links object to event(s)."""@en ;
            rdfs:label "isObjectOf"@en .


###  http://www.semanticweb.org/luciapifferi/ontologies/2020/semantic_web_exam/narratives#isParticipantOf
:isParticipantOf rdf:type owl:ObjectProperty ;
                 rdfs:domain :Participant ;
                 rdfs:range :Event ;
                 rdfs:comment """A partecipant is the participant of one or more events.
This object property links participant and event(s)."""@en ;
                 rdfs:label "isParticipantOf"@en .


###  http://www.semanticweb.org/luciapifferi/ontologies/2020/semantic_web_exam/narratives#isPublisherOf
:isPublisherOf rdf:type owl:ObjectProperty ,
                        owl:InverseFunctionalProperty ;
               rdfs:domain :Publisher ;
               rdfs:range :Book ;
               rdfs:comment """A publisher is the publisher of one or more books (so this property is not functional). But a book can only have a publisher, so this property is inverse functional.
This object property links publisher to book(s)."""@en ;
               rdfs:label "isPublisherOf"@en .


###  http://www.semanticweb.org/luciapifferi/ontologies/2020/semantic_web_exam/narratives#isReportedIn
:isReportedIn rdf:type owl:ObjectProperty ;
              owl:inverseOf :reports ;
              rdfs:domain :Narrative ;
              rdfs:range :Book ;
              rdfs:comment """It's reasonable to think that a narrative is reported in one or more books.
This object property links narrative and book(s)."""@en ;
              rdfs:label "isReportedIn"@en .


###  http://www.semanticweb.org/luciapifferi/ontologies/2020/semantic_web_exam/narratives#occursIn
:occursIn rdf:type owl:ObjectProperty ,
                   owl:FunctionalProperty ;
          rdfs:domain :Event ;
          rdfs:range :Location ;
          rdfs:comment """An event occurs in exactly one location, so this property is functional. 
This object property links event and location."""@en ;
          rdfs:label "occursIn"@en .


###  http://www.semanticweb.org/luciapifferi/ontologies/2020/semantic_web_exam/narratives#reports
:reports rdf:type owl:ObjectProperty ;
         rdfs:domain :Book ;
         rdfs:range :Narrative ;
         rdfs:comment """A book reports one or more narratives.
This object property links book and narrative(s)."""@en ;
         rdfs:label "reports"@en .


#################################################################
#    Data properties
#################################################################

###  http://www.semanticweb.org/luciapifferi/ontologies/2020/semantic_web_exam/narratives#hasBeginning
:hasBeginning rdf:type owl:DatatypeProperty ,
                       owl:FunctionalProperty ;
              rdfs:domain :Event ;
              rdfs:range xsd:dateTime ;
              rdfs:comment "An event has exactly one beginning, represented as a datetime using the appropriate XSD datatype."@en ;
              rdfs:label "hasBeginning"@en .


###  http://www.semanticweb.org/luciapifferi/ontologies/2020/semantic_web_exam/narratives#hasCharacterName
:hasCharacterName rdf:type owl:DatatypeProperty ;
                  rdfs:subPropertyOf :hasName ;
                  rdfs:domain :Character ;
                  rdfs:range xsd:string ;
                  rdfs:comment "A character can have one or more names, represented as strings."@en ;
                  rdfs:label "hasCharacterName"@en .


###  http://www.semanticweb.org/luciapifferi/ontologies/2020/semantic_web_exam/narratives#hasEnding
:hasEnding rdf:type owl:DatatypeProperty ,
                    owl:FunctionalProperty ;
           rdfs:domain :Event ;
           rdfs:range xsd:dateTime ;
           rdfs:comment "An event has exactly one ending, represented as a datetime using the appropriate XSD datatype."@en ;
           rdfs:label "hasEnding"@en .


###  http://www.semanticweb.org/luciapifferi/ontologies/2020/semantic_web_exam/narratives#hasISBNcode
:hasISBNcode rdf:type owl:DatatypeProperty ,
                      owl:FunctionalProperty ;
             rdfs:domain :Book ;
             rdfs:range xsd:string ;
             rdfs:comment "A book is identified by an ISBN code, represented as a string. A book can have only one ISBN, so this data property is functional."@en ;
             rdfs:label "hasISBNcode"@en .


###  http://www.semanticweb.org/luciapifferi/ontologies/2020/semantic_web_exam/narratives#hasLocationName
:hasLocationName rdf:type owl:DatatypeProperty ;
                 rdfs:subPropertyOf :hasName ;
                 rdfs:domain :Location ;
                 rdfs:range xsd:string ;
                 rdfs:comment "A location can have one or more names, represented as strings."@en ;
                 rdfs:label "hasLocationName"@en .


###  http://www.semanticweb.org/luciapifferi/ontologies/2020/semantic_web_exam/narratives#hasName
:hasName rdf:type owl:DatatypeProperty ;
         rdfs:range xsd:string ;
         rdfs:comment "A resource can have one or more names, represented as strings."@en ;
         rdfs:label "hasName"@en .


###  http://www.semanticweb.org/luciapifferi/ontologies/2020/semantic_web_exam/narratives#hasTitle
:hasTitle rdf:type owl:DatatypeProperty ;
          rdfs:domain :Book ;
          rdfs:range xsd:string ;
          rdfs:comment "A book has one or more title. This data property links book to one or more strings."@en ;
          rdfs:label "hasTitle"@en .


#################################################################
#    Classes
#################################################################

###  http://www.semanticweb.org/luciapifferi/ontologies/2020/semantic_web_exam/narratives#Book
:Book rdf:type owl:Class ;
      rdfs:subClassOf [ rdf:type owl:Restriction ;
                        owl:onProperty :reports ;
                        owl:minQualifiedCardinality "1"^^xsd:nonNegativeInteger ;
                        owl:onClass :Narrative
                      ] ,
                      [ rdf:type owl:Restriction ;
                        owl:onProperty :hasPublisher ;
                        owl:qualifiedCardinality "1"^^xsd:nonNegativeInteger ;
                        owl:onClass :Publisher
                      ] ,
                      [ rdf:type owl:Restriction ;
                        owl:onProperty :hasTitle ;
                        owl:someValuesFrom xsd:string
                      ] ,
                      [ rdf:type owl:Restriction ;
                        owl:onProperty :hasISBNcode ;
                        owl:qualifiedCardinality "1"^^xsd:nonNegativeInteger ;
                        owl:onDataRange xsd:string
                      ] ;
      rdfs:comment "A book is a resource that reports one or more narratives. It also has a title and it is identified by an ISBN code. Furthermore, it has exactly one publisher."@en ;
      rdfs:label "Book"@en .


###  http://www.semanticweb.org/luciapifferi/ontologies/2020/semantic_web_exam/narratives#Character
:Character rdf:type owl:Class ;
           rdfs:subClassOf :Participant ,
                           [ rdf:type owl:Restriction ;
                             owl:onProperty :hasCharacterName ;
                             owl:someValuesFrom xsd:string
                           ] ;
           owl:disjointWith :Object ;
           owl:disjointUnionOf ( :Human
                                 :NotHuman
                               ) ;
           rdfs:comment "A resource that can participate to an event and has a name. Furthermore a character can be human or not human."@en ;
           rdfs:label "Character"@en .


###  http://www.semanticweb.org/luciapifferi/ontologies/2020/semantic_web_exam/narratives#Event
:Event rdf:type owl:Class ;
       rdfs:subClassOf [ rdf:type owl:Restriction ;
                         owl:onProperty :hasParticipant ;
                         owl:minQualifiedCardinality "1"^^xsd:nonNegativeInteger ;
                         owl:onClass :Participant
                       ] ,
                       [ rdf:type owl:Restriction ;
                         owl:onProperty :occursIn ;
                         owl:qualifiedCardinality "1"^^xsd:nonNegativeInteger ;
                         owl:onClass :Location
                       ] ,
                       [ rdf:type owl:Restriction ;
                         owl:onProperty :hasBeginning ;
                         owl:qualifiedCardinality "1"^^xsd:nonNegativeInteger ;
                         owl:onDataRange xsd:dateTime
                       ] ,
                       [ rdf:type owl:Restriction ;
                         owl:onProperty :hasEnding ;
                         owl:qualifiedCardinality "1"^^xsd:nonNegativeInteger ;
                         owl:onDataRange xsd:dateTime
                       ] ;
       rdfs:comment "One or more events compose a narrative and each event occurs in exactly one location and has exactly one beginning and one ending. Furthermore each event has at least one participating character or object."@en ;
       rdfs:label "Event"@en .


###  http://www.semanticweb.org/luciapifferi/ontologies/2020/semantic_web_exam/narratives#FictionalLocation
:FictionalLocation rdf:type owl:Class ;
                   rdfs:subClassOf :Location ;
                   owl:disjointWith :RealLocation ;
                   rdfs:comment "A specific type of location that is fictional."@en ;
                   rdfs:label "FictionalLocation"@en .


###  http://www.semanticweb.org/luciapifferi/ontologies/2020/semantic_web_exam/narratives#Human
:Human rdf:type owl:Class ;
       rdfs:subClassOf :Character ;
       owl:disjointWith :NotHuman ;
       rdfs:comment "A specific type of character that is human."@en ;
       rdfs:label "HumanCharacter"@en .


###  http://www.semanticweb.org/luciapifferi/ontologies/2020/semantic_web_exam/narratives#Location
:Location rdf:type owl:Class ;
          rdfs:subClassOf [ rdf:type owl:Restriction ;
                            owl:onProperty :hasLocationName ;
                            owl:someValuesFrom xsd:string
                          ] ;
          owl:disjointUnionOf ( :FictionalLocation
                                :RealLocation
                              ) ;
          rdfs:comment "A location hosts one or more events. Each location has a name and can be a real location or a fictional location."@en ;
          rdfs:label "Location"@en .


###  http://www.semanticweb.org/luciapifferi/ontologies/2020/semantic_web_exam/narratives#Narrative
:Narrative rdf:type owl:Class ;
           rdfs:subClassOf [ rdf:type owl:Restriction ;
                             owl:onProperty :isComposedOf ;
                             owl:allValuesFrom :Event
                           ] ,
                           [ rdf:type owl:Restriction ;
                             owl:onProperty :isComposedOf ;
                             owl:minQualifiedCardinality "1"^^xsd:nonNegativeInteger ;
                             owl:onClass :Event
                           ] ,
                           [ rdf:type owl:Restriction ;
                             owl:onProperty :isCreatedBy ;
                             owl:minQualifiedCardinality "1"^^xsd:nonNegativeInteger ;
                             owl:onClass :Narrator
                           ] ;
           rdfs:comment "A narrative is exclusively composed of one or more events. Each narrative is created by at least one narrator and is reported in a book."@en ;
           rdfs:label "Narrative"@en .


###  http://www.semanticweb.org/luciapifferi/ontologies/2020/semantic_web_exam/narratives#Narrator
:Narrator rdf:type owl:Class ;
          rdfs:comment "A narrator is the creator of a narrative."@en ;
          rdfs:label "Narrator"@en .


###  http://www.semanticweb.org/luciapifferi/ontologies/2020/semantic_web_exam/narratives#NotHuman
:NotHuman rdf:type owl:Class ;
          rdfs:subClassOf :Character ;
          rdfs:comment "A specific type of character that is not human."@en ;
          rdfs:label "NotHumanCharacter"@en .


###  http://www.semanticweb.org/luciapifferi/ontologies/2020/semantic_web_exam/narratives#Object
:Object rdf:type owl:Class ;
        rdfs:subClassOf :Participant ;
        rdfs:comment "A resource that can participate to an event."@en ;
        rdfs:label "Object"@en .


###  http://www.semanticweb.org/luciapifferi/ontologies/2020/semantic_web_exam/narratives#Organisation
:Organisation rdf:type owl:Class ;
              rdfs:comment "An organized group of people (such as publishers) with a particular purpose."@en ;
              rdfs:label "Organisation"@en .


###  http://www.semanticweb.org/luciapifferi/ontologies/2020/semantic_web_exam/narratives#Participant
:Participant rdf:type owl:Class ;
             owl:disjointUnionOf ( :Character
                                   :Object
                                 ) ;
             rdfs:comment "A resource who participate to an event and that can be a character or a object."@en ;
             rdfs:label "Participant"@en .


###  http://www.semanticweb.org/luciapifferi/ontologies/2020/semantic_web_exam/narratives#Publisher
:Publisher rdf:type owl:Class ;
           rdfs:subClassOf :Organisation ;
           rdfs:comment "A resource responsible for publishing a book."@en ;
           rdfs:label "Publisher"@en .


###  http://www.semanticweb.org/luciapifferi/ontologies/2020/semantic_web_exam/narratives#RealLocation
:RealLocation rdf:type owl:Class ;
              rdfs:subClassOf :Location ;
              rdfs:comment "A specific type of location that is real."@en ;
              rdfs:label "RealLocation"@en .


#################################################################
#    Individuals
#################################################################

###  http://www.semanticweb.org/luciapifferi/ontologies/2020/semantic_web_exam/narratives#book1
:book1 rdf:type owl:NamedIndividual ,
                :Book ;
       :hasPublisher :publisher1 ;
       :reports :narrative1 ,
                :narrative3 ;
       :hasISBNcode "978-3-16-148410-0"^^xsd:string ;
       :hasTitle "Titolo1"^^xsd:string .


###  http://www.semanticweb.org/luciapifferi/ontologies/2020/semantic_web_exam/narratives#book2
:book2 rdf:type owl:NamedIndividual ,
                :Book ;
       :hasPublisher :publisher2 ;
       :reports :narrative2 ,
                :narrative3 ;
       :hasISBNcode "978-88-17-07926-6"^^xsd:string ;
       :hasTitle "Titolo2"^^xsd:string .


###  http://www.semanticweb.org/luciapifferi/ontologies/2020/semantic_web_exam/narratives#event1
:event1 rdf:type owl:NamedIndividual ,
                 :Event ;
        :compose :narrative1 ;
        :hasParticipant :participant1 ,
                        :participant2 ;
        :occursIn :fictionalLocation1 ;
        :hasBeginning "2016-01-01T00:00:00"^^xsd:dateTime ;
        :hasEnding "2017-02-01T00:00:00"^^xsd:dateTime .


###  http://www.semanticweb.org/luciapifferi/ontologies/2020/semantic_web_exam/narratives#event2
:event2 rdf:type owl:NamedIndividual ,
                 :Event ;
        :compose :narrative2 ;
        :hasParticipant :participant3 ,
                        :participant4 ;
        :occursIn :fictionalLocation1 ;
        :hasBeginning "2018-02-01T00:00:00"^^xsd:dateTime ;
        :hasEnding "2019-02-01T00:00:00"^^xsd:dateTime .


###  http://www.semanticweb.org/luciapifferi/ontologies/2020/semantic_web_exam/narratives#event3
:event3 rdf:type owl:NamedIndividual ,
                 :Event ;
        :hasCharacter :participant6 ;
        :hasObject :participant5 ;
        :occursIn :realLocation1 ;
        :hasBeginning "2017-03-01T00:00:00"^^xsd:dateTime ;
        :hasEnding "2017-05-01T00:00:00"^^xsd:dateTime .


###  http://www.semanticweb.org/luciapifferi/ontologies/2020/semantic_web_exam/narratives#event4
:event4 rdf:type owl:NamedIndividual ,
                 :Event ;
        :hasCharacter :participant7 ,
                      :participant8 ;
        :occursIn :realLocation1 ;
        :hasBeginning "2018-02-01T00:00:00"^^xsd:dateTime ;
        :hasEnding "2018-05-01T00:00:00"^^xsd:dateTime .


###  http://www.semanticweb.org/luciapifferi/ontologies/2020/semantic_web_exam/narratives#event5
:event5 rdf:type owl:NamedIndividual ,
                 :Event ;
        :hasCharacter :participant3 ,
                      :participant4 ;
        :occursIn :fictionalLocation2 ;
        :hasBeginning "2018-01-01T00:00:00"^^xsd:dateTime ;
        :hasEnding "2020-01-08T00:00:00"^^xsd:dateTime .


###  http://www.semanticweb.org/luciapifferi/ontologies/2020/semantic_web_exam/narratives#event6
:event6 rdf:type owl:NamedIndividual ,
                 :Event ;
        :hasCharacter :participant3 ;
        :hasObject :participant2 ;
        :occursIn :realLocation2 ;
        :hasBeginning "2017-07-01T00:00:00"^^xsd:dateTime ;
        :hasEnding "2017-08-01T00:00:00"^^xsd:dateTime .


###  http://www.semanticweb.org/luciapifferi/ontologies/2020/semantic_web_exam/narratives#fictionalLocation1
:fictionalLocation1 rdf:type owl:NamedIndividual ,
                             :FictionalLocation ;
                    :hosts :event1 ,
                           :event2 ;
                    :hasLocationName "Narnia"^^xsd:string .


###  http://www.semanticweb.org/luciapifferi/ontologies/2020/semantic_web_exam/narratives#fictionalLocation2
:fictionalLocation2 rdf:type owl:NamedIndividual ,
                             :FictionalLocation ;
                    :hasLocationName "Lilliput"^^xsd:string .


###  http://www.semanticweb.org/luciapifferi/ontologies/2020/semantic_web_exam/narratives#narrative1
:narrative1 rdf:type owl:NamedIndividual ,
                     :Narrative ;
            :isComposedOf :event1 ,
                          :event3 ;
            :isCreatedBy :narrator1 ,
                         :narrator2 ;
            :isReportedIn :book1 .


###  http://www.semanticweb.org/luciapifferi/ontologies/2020/semantic_web_exam/narratives#narrative2
:narrative2 rdf:type owl:NamedIndividual ,
                     :Narrative ;
            :isComposedOf :event2 ,
                          :event4 ;
            :isCreatedBy :narrator2 ,
                         :narrator3 ;
            :isReportedIn :book2 .


###  http://www.semanticweb.org/luciapifferi/ontologies/2020/semantic_web_exam/narratives#narrative3
:narrative3 rdf:type owl:NamedIndividual ,
                     :Narrative ;
            :isComposedOf :event5 ,
                          :event6 ;
            :isCreatedBy :narrator1 ,
                         :narrator3 ;
            :isReportedIn :book1 ,
                          :book2 .


###  http://www.semanticweb.org/luciapifferi/ontologies/2020/semantic_web_exam/narratives#narrator1
:narrator1 rdf:type owl:NamedIndividual ,
                    :Narrator ;
           :collaborates :publisher1 ;
           :creates :narrative1 .


###  http://www.semanticweb.org/luciapifferi/ontologies/2020/semantic_web_exam/narratives#narrator2
:narrator2 rdf:type owl:NamedIndividual ,
                    :Narrator ;
           :creates :narrative1 .


###  http://www.semanticweb.org/luciapifferi/ontologies/2020/semantic_web_exam/narratives#narrator3
:narrator3 rdf:type owl:NamedIndividual ,
                    :Narrator .


###  http://www.semanticweb.org/luciapifferi/ontologies/2020/semantic_web_exam/narratives#participant1
:participant1 rdf:type owl:NamedIndividual ,
                       :Human ;
              :isCharacterOf :event1 ;
              :hasCharacterName "Luigi"^^xsd:string .


###  http://www.semanticweb.org/luciapifferi/ontologies/2020/semantic_web_exam/narratives#participant2
:participant2 rdf:type owl:NamedIndividual ,
                       :Object ;
              :isObjectOf :event1 .


###  http://www.semanticweb.org/luciapifferi/ontologies/2020/semantic_web_exam/narratives#participant3
:participant3 rdf:type owl:NamedIndividual ,
                       :NotHuman ;
              :isCharacterOf :event2 ;
              :hasCharacterName "Pluto"^^xsd:string .


###  http://www.semanticweb.org/luciapifferi/ontologies/2020/semantic_web_exam/narratives#participant4
:participant4 rdf:type owl:NamedIndividual ,
                       :NotHuman ;
              :isCharacterOf :event2 ;
              :hasCharacterName "Paperino"^^xsd:string .


###  http://www.semanticweb.org/luciapifferi/ontologies/2020/semantic_web_exam/narratives#participant5
:participant5 rdf:type owl:NamedIndividual ,
                       :Object .


###  http://www.semanticweb.org/luciapifferi/ontologies/2020/semantic_web_exam/narratives#participant6
:participant6 rdf:type owl:NamedIndividual ,
                       :NotHuman ;
              :hasCharacterName "Topolino"^^xsd:string .


###  http://www.semanticweb.org/luciapifferi/ontologies/2020/semantic_web_exam/narratives#participant7
:participant7 rdf:type owl:NamedIndividual ,
                       :Human ;
              :hasCharacterName "Maria"^^xsd:string .


###  http://www.semanticweb.org/luciapifferi/ontologies/2020/semantic_web_exam/narratives#participant8
:participant8 rdf:type owl:NamedIndividual ,
                       :Human ;
              :isParticipantOf :event4 ;
              :hasCharacterName "Giuseppe"^^xsd:string .


###  http://www.semanticweb.org/luciapifferi/ontologies/2020/semantic_web_exam/narratives#publisher1
:publisher1 rdf:type owl:NamedIndividual ,
                     :Publisher ;
            :isPublisherOf :book1 .


###  http://www.semanticweb.org/luciapifferi/ontologies/2020/semantic_web_exam/narratives#publisher2
:publisher2 rdf:type owl:NamedIndividual ,
                     :Publisher ;
            :isPublisherOf :book2 .


###  http://www.semanticweb.org/luciapifferi/ontologies/2020/semantic_web_exam/narratives#realLocation1
:realLocation1 rdf:type owl:NamedIndividual ,
                        :RealLocation ;
               :hasLocationName "Pisa"^^xsd:string .


###  http://www.semanticweb.org/luciapifferi/ontologies/2020/semantic_web_exam/narratives#realLocation2
:realLocation2 rdf:type owl:NamedIndividual ,
                        :RealLocation ;
               :hasLocationName "Lucca"^^xsd:string .


#################################################################
#    General axioms
#################################################################

[ rdf:type owl:AllDisjointClasses ;
  owl:members ( :Book
                :Event
                :Location
                :Narrative
                :Narrator
                :Organisation
                :Participant
              )
] .


[ rdf:type owl:AllDifferent ;
  owl:distinctMembers ( :book1
                        :book2
                      )
] .


[ rdf:type owl:AllDifferent ;
  owl:distinctMembers ( :event1
                        :event2
                        :event3
                        :event4
                        :event5
                        :event6
                      )
] .


[ rdf:type owl:AllDifferent ;
  owl:distinctMembers ( :fictionalLocation1
                        :fictionalLocation2
                      )
] .


[ rdf:type owl:AllDifferent ;
  owl:distinctMembers ( :narrative1
                        :narrative2
                        :narrative3
                      )
] .


[ rdf:type owl:AllDifferent ;
  owl:distinctMembers ( :narrator1
                        :narrator2
                        :narrator3
                      )
] .


[ rdf:type owl:AllDifferent ;
  owl:distinctMembers ( :participant1
                        :participant2
                        :participant3
                        :participant4
                        :participant5
                        :participant6
                        :participant7
                        :participant8
                      )
] .


[ rdf:type owl:AllDifferent ;
  owl:distinctMembers ( :publisher1
                        :publisher2
                      )
] .


[ rdf:type owl:AllDifferent ;
  owl:distinctMembers ( :realLocation1
                        :realLocation2
                      )
] .


###  Generated by the OWL API (version 4.5.9.2019-02-01T07:24:44Z) https://github.com/owlcs/owlapi
